lib/Array.v
@@ -12,21 +12,18 @@ Parameter array : Type -> Type.
 
 Parameter length : forall T, array T -> nat.
 
-Parameter read : forall T, array T -> nat -> option T.
+Parameter read : forall T `{Inhab T}, array T -> nat -> T.
 Parameter write : forall T, array T -> nat -> T -> array T.
 
 Parameter from_list : forall T, list T -> array T.
 Parameter to_list : forall T, array T -> list T.
 
-Parameter read_defined : forall T (a : array T) n,
+Parameter read_write_eq : forall T `{Inhab T} a (t : T) n,
   n < length a ->
-  exists t, read a n = Some t.
+  read (write a n t) n = t.
 
-Parameter read_write_eq : forall T a (t : T) n,
-  n < length a ->
-  read (write a n t) n = Some t.
-
-Parameter read_write_neq : forall T a (t : T) n1 n2,
+Parameter read_write_neq : forall T `{Inhab T} a (t : T) n1 n2,
+  n2 < length a ->
   n1 <> n2 ->
   read (write a n1 t) n2 = read a n2.
 
@@ -39,74 +36,56 @@ Parameter from_list_length : forall T (l : list T),
 Parameter to_list_length : forall T (a : array T),
   LibList.length (to_list a) = length a.
 
-Parameter from_list_read : forall T (l : list T) n,
-  read (from_list l) n = nth_option n l.
+Parameter from_list_read : forall T `{Inhab T} (l : list T) n,
+  read (from_list l) n = nth n l.
 
-Parameter to_list_read : forall T (a : array T) n,
-  nth_option n (to_list a) = read a n.
+Parameter to_list_read : forall T `{Inhab T} (a : array T) n,
+  nth n (to_list a) = read a n.
 
 End ArraySpec.
 
-Module Array : ArraySpec.
+(* FIXME: If I mask the types with the module type annotation below, I get a universe inconsistency in State.v. *)
+Module ArrayList (*: ArraySpec*).
 
 Definition array := list.
 
 Definition length T := length : array T -> nat.
 
-Definition read T (a : array T) n := nth_option n a.
-Definition write T a n (t : T) := update n t a.
+Definition read T `{Inhab T} (a : array T) n := nth n a.
+Definition write T (a : array T) n t := update n t a : array T.
 
 Definition from_list T := id : list T -> array T.
 Definition to_list T := id : array T -> list T.
 
-
-Lemma read_defined : forall T (a : array T) n,
+Lemma read_write_eq : forall T `{Inhab T} a (t : T) n,
   n < length a ->
-  exists t, read a n = Some t.
-Proof.
-  introv I. destruct (read a n) eqn: E.
-  - exists*.
-  - apply nth_option_length in E. unfolds length. nat_math.
-Qed.
+  read (write a n t) n = t.
+Proof. introv I. apply nth_update_eq. unfolds length. nat_math. Qed.
 
-Lemma read_write_eq : forall T a (t : T) n,
-  n < length a ->
-  read (write a n t) n = Some t.
-Proof.
-  introv I. destruct (read a n) eqn: E.
-  - apply nth_option_defined in E. rewrite nth_update_eq.
-  - apply nth_option_length in E. unfolds length. nat_math.
-Qed.
-
-Lemma read_write_neq : forall T a (t : T) n1 n2,
+Lemma read_write_neq : forall T `{Inhab T} a (t : T) n1 n2,
+  n2 < length a ->
   n1 <> n2 ->
   read (write a n1 t) n2 = read a n2.
-Proof.
-Qed.
+Proof. introv I D. applys nth_update_neq D. unfolds length. nat_math. Qed.
 
 Lemma write_length : forall T a (t : T) n,
   length (write a n t) = length a.
-Proof.
-Qed.
+Proof. introv. apply length_update. Qed.
 
 Lemma from_list_length : forall T (l : list T),
   length (from_list l) = LibList.length l.
-Proof.
-Qed.
+Proof. reflexivity. Qed.
 
 Lemma to_list_length : forall T (a : array T),
   LibList.length (to_list a) = length a.
-Proof.
-Qed.
+Proof. reflexivity. Qed.
 
-Lemma from_list_read : forall T (l : list T) n,
-  read (from_list l) n = nth_option n l.
-Proof.
-Qed.
+Lemma from_list_read : forall T `{Inhab T} (l : list T) n,
+  read (from_list l) n = nth n l.
+Proof. reflexivity. Qed.
 
-Lemma to_list_read : forall T (a : array T) n,
-  nth_option n (to_list a) = read a n.
-Proof.
-Qed.
+Lemma to_list_read : forall T `{Inhab T} (a : array T) n,
+  nth n (to_list a) = read a n.
+Proof. reflexivity. Qed.
 
-End Array.
+End ArrayList.
